Steel.List: Derived + Impl
+ Steel.Util: vexists

steel/Learn.Steel.List.Data.fsti
@@ -33,7 +33,7 @@ val __end_sg_entry : unit
 
 
 type mlist_sel_t (#a : Type) (entry : ref (cell a)) (len : nat) (exit : ref (cell a)) =
-  l:list (ref (cell a) & a){L.length l = len /\ sg_entry l exit == entry}
+  l : list (ref (cell a) & a){L.length l = len /\ sg_entry l exit == entry}
 
 val mlist_sel (#a : Type) (entry : ref (cell a)) (len : nat) (exit : ref (cell a))
   : selector (mlist_sel_t entry len exit) (mlist_sl #a entry len exit)
@@ -53,20 +53,33 @@ unfold let mlist (#a : Type) (entry : ref (cell a)) ([@@@smt_fallback] len : nat
 [@@ __steel_reduce__]
 let sel_list (#a:Type0) (#p:vprop) (entry:ref (cell a)) (len : nat) (exit : ref (cell a))
   (h:rmem p{FStar.Tactics.with_tactic selector_tactic (can_be_split p (mlist entry len exit) /\ True)})
-  : GTot (list (ref (cell a) & a))
+  : GTot (mlist_sel_t #a entry len exit)
   = h (mlist entry len exit)
 
 (* intro/elim lemmas *)
+
+val intro_mlist_nil_lem (#a : Type) (r0 : ref (cell a)) (m : mem)
+  : Lemma (ensures  interp (hp_of (mlist r0 0 r0)) m /\
+                    mlist_sel r0 0 r0 m == [])
 
 val intro_mlist_nil (#a : Type) (#opened:inames) (r0 : ref (cell a))
   : SteelGhost unit opened
       emp (fun () -> mlist r0 0 r0)
       (requires fun _ -> True) (ensures fun _ () h1 -> sel_list r0 0 r0 h1 == [])
 
+val elim_mlist_nil_lem (#a : Type) (r0 r1 : ref (cell a)) (m : mem)
+  : Lemma (requires interp (hp_of (mlist r0 0 r1)) m)
+          (ensures  interp (hp_of emp) m /\ r0 == r1)
+
 val elim_mlist_nil (#a : Type) (#opened:inames) (r0 : ref (cell a)) (r1 : ref (cell a))
   : SteelGhost unit opened
       (mlist r0 0 r1) (fun () -> emp)
       (requires fun _ -> True) (ensures fun _ () _ -> r0 == r1)
+
+val intro_mlist_cons_lem (#a : Type) (r0 r1 : ref (cell a)) (x : a) (len : nat) (exit : ref (cell a)) (m : mem)
+  : Lemma (requires interp (hp_of (pts_to r0 full_perm ({next = r1; data = x}) `star` mlist r1 len exit)) m)
+          (ensures  interp (hp_of (mlist r0 (len + 1) exit)) m /\
+                    mlist_sel r0 (len + 1) exit m == (r0, x) :: mlist_sel r1 len exit m)
 
 val intro_mlist_cons' (#a : Type) (#opened:inames) (r0 r1 : ref (cell a)) (x : a) (len : nat) (exit : ref (cell a))
   : SteelGhost unit opened
@@ -83,6 +96,14 @@ val intro_mlist_cons (#a : Type) (#opened:inames) (r0 r1 : ref (cell a)) (len : 
      (ensures  fun h0 () h1 -> sel_list r0 (len + 1) exit h1
                             == (r0, (sel r0 h0).data) :: sel_list r1 len exit h0)
 
+val elim_mlist_cons_lem (#a : Type) (r0 : ref (cell a)) (hd : ref (cell a) & a) (tl : list (ref (cell a) & a))
+                        (len : nat) (exit : ref (cell a)) (m: mem)
+  : Lemma (requires interp (hp_of (mlist r0 (len + 1) exit)) m /\ mlist_sel r0 (len + 1) exit m == hd :: tl)
+          (ensures (let r1 = sg_entry tl exit in
+                    let q  = pts_to r0 full_perm ({next = r1; data = hd._2}) `star` mlist r1 len exit in
+                    interp (hp_of q) m /\
+                    (sel_of q m <: unit & mlist_sel_t r1 len exit) == ((), tl)))
+
 val elim_mlist_cons (#a : Type) (#opened:inames) (r0 : ref (cell a)) (len : nat) (exit : ref (cell a))
   : SteelGhost (G.erased (ref (cell a))) opened
      (mlist r0 (len + 1) exit)
@@ -90,5 +111,6 @@ val elim_mlist_cons (#a : Type) (#opened:inames) (r0 : ref (cell a)) (len : nat)
      (requires fun _ -> True)
      (ensures  fun h0 r1 h1 ->
       (let l = sel_list r0 (len+1) exit h0 in
+       G.reveal r1 == sg_entry (L.tl l) exit /\ (* also implied by [sel_list r1 len exit h1 == L.tl l] *)
        sel r0 h1 == {next = r1; data = (L.hd l)._2} /\
        sel_list r1 len exit h1 == L.tl l))
