steel/Learn.Steel.List.Derived.fst
@@ -1,98 +1,27 @@
 module Learn.Steel.List.Derived
 
-module L = FStar.List.Pure
-module G = FStar.Ghost
+let v (#a:Type) (entry : ref (cell a)) (len : nat)
+  = mlist #a entry len null
 
-open Steel.Memory
-open Steel.Effect
-open Steel.Effect.Atomic
-open Steel.Reference
+let f (#a:Type) (entry : ref (cell a)) (len : nat) (l : t_of (v entry len)) : mlistN_sel_t #a entry
+  = l
 
-open Learn.Steel.List.DataD
-open Learn.Steel.List.Data
+let mlistN_sl #a (entry : ref (cell a)) =
+  US.vexists_sl (v #a entry)
 
+let mlistN_indep #a (entry : ref (cell a))
+  : Lemma (ensures US.vexists_indep (v entry) #(mlistN_sel_t entry) (f entry))
+  = US.vexists_indepI_unique (v entry) (mlistN_length_unique entry)
 
-let mlist_rew_len #a #opened entry len0 len1 exit
-  : SteelGhost unit opened
-    (mlist #a entry len0 exit) (fun () -> mlist #a entry len1 exit)
-    (requires fun _ -> len0 = len1)
-    (ensures  fun h0 () h1 -> sel_list entry len0 exit h0 == sel_list entry len1 exit h1)
-  = change_equal_slprop
-       (mlist entry len0 exit) (mlist entry len1 exit)
+let mlistN_sel #a (entry : ref (cell a)) =
+  mlistN_indep entry;
+  US.vexists_sel (v #a entry) #(mlistN_sel_t entry) (f #a entry)
 
+let intro_mlistN #a #opened entry len =
+  mlistN_indep entry;
+  US.intro_vexists len (v entry) #(mlistN_sel_t entry) (f entry)
 
-let entry_not_null #a #opened entry len exit
-  : SteelGhost unit opened
-      (mlist #a entry len exit) (fun () -> mlist #a entry len exit)
-      (requires fun _        -> len > 0)
-      (ensures  fun h0 () h1 -> frame_equalities (mlist #a entry len exit) h0 h1 /\
-                             is_null entry == false)
+let elim_mlistN (#a:Type) (#opened:inames) (entry:ref (cell a))
   =
-    mlist_rew_len entry len ((len-1)+1) exit;
-    let r1 = elim_mlist_cons entry (len - 1) exit in
-    vptr_not_null entry;
-    intro_mlist_cons entry r1 (len - 1) exit;
-    mlist_rew_len entry ((len-1)+1) len exit
-
-
-let intro_mlist_sglt #a #opened r0 exit
-  : SteelGhost unit opened
-      (vptr r0) (fun () -> mlist #a r0 1 exit)
-      (requires fun h0       -> (sel r0 h0).next == exit)
-      (ensures  fun h0 () h1 -> sel_list r0 1 exit h1 == [r0, (sel r0 h0).data])
-  =
-    intro_mlist_nil exit;
-    intro_mlist_cons r0 exit 0 exit
-
-
-let rec intro_mlist_append #a #opened r0 (len0 : nat) r1 (len1 : nat) r2
-  : SteelGhost unit opened
-      (mlist #a r0 len0 r1 `star` mlist #a r1 len1 r2)
-      (fun () -> mlist #a r0 (len0+len1) r2)
-      (requires fun _ -> True)
-      (ensures  fun h0 () h1 ->
-        sel_list r0 (len0+len1) r2 h1 == L.(sel_list r0 len0 r1 h0 @ sel_list r1 len1 r2 h0))
-      (decreases len0)
-  =
-    if len0 = 0
-    then begin
-        mlist_rew_len r0 len0 0 r1;
-      elim_mlist_nil r0 r1;
-      change_equal_slprop (mlist r1 len1 r2) (mlist r0 (len0+len1) r2)
-    end else begin
-      let len0' = len0 - 1 in
-        mlist_rew_len r0 len0 (len0'+1) r1;
-      let r0' = elim_mlist_cons r0 len0' r1 in
-      intro_mlist_append r0' len0' r1 len1 r2;
-      intro_mlist_cons r0 r0' (len0'+len1) r2;
-        mlist_rew_len r0 ((len0'+len1)+1) (len0+len1) r2
-    end
-
-let rec elim_mlist_append #a #opened r0 (len len0 len1 : nat) r2 (l0 l1 : list (ref (cell a) & a))
-  : SteelGhost (G.erased (ref (cell a))) opened
-      (mlist r0 len r2)
-      (fun r1 -> mlist r0 len0 r1 `star` mlist r1 len1 r2)
-      (requires fun h0 ->
-        sel_list r0 len r2 h0 == L.(l0@l1) /\
-        L.length l0 = len0 /\ L.length l1 = len1)
-      (ensures  fun _ r1 h1 ->
-        sel_list r0 len0 r1 h1 == l0 /\
-        sel_list r1 len1 r2 h1 == l1)
-      (decreases len0)
-  =
-    if len0 = 0
-    then begin
-      intro_mlist_nil r0;
-        mlist_rew_len r0 0 len0 r0;
-      change_equal_slprop (mlist r0 len r2) (mlist r0 len1 r2);
-      r0
-    end else begin
-      let len'  = len  - 1 in
-      let len0' = len0 - 1 in
-        mlist_rew_len r0 len (len'+1) r2;
-      let r0' = elim_mlist_cons r0 len' r2 in
-      let r1  = elim_mlist_append r0' len' len0' len1 r2 (L.tl l0) l1 in
-      intro_mlist_cons r0 r0' len0' r1;
-        mlist_rew_len r0 (len0'+1) len0 r1;
-      r1
-    end
+    mlistN_indep entry;
+    US.witness_vexists #nat (v entry) #(mlistN_sel_t entry) (f entry)
