steel/Learn.Steel.List.Derived.fsti
@@ -1,0 +1,289 @@
+module Learn.Steel.List.Derived
+
+module L  = FStar.List.Pure
+module G  = FStar.Ghost
+module US = Learn.Steel.Util
+
+open Steel.Memory
+open Steel.Effect
+open Steel.Effect.Atomic
+open Steel.FractionalPermission
+open Steel.Reference
+
+open Learn.Steel.List.DataD
+open Learn.Steel.List.Data
+
+
+let entry_not_null_lem #a entry len exit m
+  : Lemma (requires interp (hp_of (mlist #a entry len exit)) m /\
+                    len > 0)
+          (ensures  is_null entry == false)
+  =
+    let hd :: tl = mlist_sel entry len exit m in
+    elim_mlist_cons_lem entry hd tl (len - 1) exit m;
+    pts_to_not_null entry full_perm ({next = sg_entry tl exit; data = hd._2}) m      
+
+(* Not true if the exit is non-null (if there is a loop) *)
+let rec mlistN_length_unique #a entry len0 len1 m
+  : Lemma (requires interp (hp_of (mlist #a entry len0 null)) m /\
+                    interp (hp_of (mlist #a entry len1 null)) m)
+          (ensures  len0 = len1)
+          (decreases len0)
+  =
+    match mlist_sel entry len0 null m, mlist_sel entry len1 null m with
+    | [], [] -> ()
+    | hd0 :: tl0, hd1 :: tl1 ->
+      elim_mlist_cons_lem entry hd0 tl0 (len0-1) null m;
+      elim_mlist_cons_lem entry hd1 tl1 (len1-1) null m;
+      US.pts_to_ref_injective_and entry full_perm
+        ({next = sg_entry tl0 null; data = hd0._2})
+        ({next = sg_entry tl1 null; data = hd1._2})
+        m;
+      assert (sg_entry tl0 null == sg_entry tl1 null);
+      mlistN_length_unique (sg_entry tl0 null) (len0-1) (len1-1) m
+    | [], _ :: _ ->
+      assert (entry == null);
+      entry_not_null_lem entry len1 null m
+    | _ :: _, [] ->
+      assert (entry == null);
+      entry_not_null_lem entry len0 null m
+
+(* Ghost lemmas *)
+
+let mlist_rew_len #a #opened entry len0 len1 exit
+  : SteelGhost unit opened
+      (mlist #a entry len0 exit) (fun () -> mlist #a entry len1 exit)
+      (requires fun _ -> len0 = len1)
+      (ensures  fun h0 () h1 -> sel_list entry len0 exit h0 == sel_list entry len1 exit h1)
+  = change_equal_slprop
+       (mlist entry len0 exit) (mlist entry len1 exit)
+
+let entry_not_null #a #opened entry len exit
+  : SteelGhost unit opened
+      (mlist #a entry len exit) (fun () -> mlist #a entry len exit)
+      (requires fun _        -> len > 0)
+      (ensures  fun h0 () h1 -> frame_equalities (mlist #a entry len exit) h0 h1 /\
+                             is_null entry == false)
+  = (* ALT : [extract_info] + [entry_not_null_lem] *)
+    mlist_rew_len entry len ((len-1)+1) exit;
+    let r1 = elim_mlist_cons entry (len - 1) exit in
+    vptr_not_null entry;
+    intro_mlist_cons entry r1 (len - 1) exit;
+    mlist_rew_len entry ((len-1)+1) len exit
+
+
+let intro_mlist_sglt #a #opened r0 exit
+  : SteelGhost unit opened
+      (vptr r0) (fun () -> mlist #a r0 1 exit)
+      (requires fun h0       -> (sel r0 h0).next == exit)
+      (ensures  fun h0 () h1 -> sel_list r0 1 exit h1 == [r0, (sel r0 h0).data])
+  =
+    intro_mlist_nil exit;
+    intro_mlist_cons r0 exit 0 exit
+
+
+let rec intro_mlist_append #a #opened r0 (len0 : nat) r1 (len1 : nat) r2
+  : SteelGhost unit opened
+      (mlist #a r0 len0 r1 `star` mlist #a r1 len1 r2)
+      (fun () -> mlist #a r0 (len0+len1) r2)
+      (requires fun _ -> True)
+      (ensures  fun h0 () h1 ->
+        sel_list r0 (len0+len1) r2 h1 == L.(sel_list r0 len0 r1 h0 @ sel_list r1 len1 r2 h0))
+      (decreases len0)
+  =
+    if len0 = 0
+    then begin
+        mlist_rew_len r0 len0 0 r1;
+      elim_mlist_nil r0 r1;
+      change_equal_slprop (mlist r1 len1 r2) (mlist r0 (len0+len1) r2)
+    end else begin
+      let len0' = len0 - 1 in
+        mlist_rew_len r0 len0 (len0'+1) r1;
+      let r0' = elim_mlist_cons r0 len0' r1 in
+      intro_mlist_append r0' len0' r1 len1 r2;
+      intro_mlist_cons r0 r0' (len0'+len1) r2;
+        mlist_rew_len r0 ((len0'+len1)+1) (len0+len1) r2
+    end
+
+let rec elim_mlist_append #a #opened r0 (len len0 len1 : nat) r2 (l0 l1 : list (ref (cell a) & a))
+  : SteelGhost (G.erased (ref (cell a))) opened
+      (mlist r0 len r2)
+      (fun r1 -> mlist r0 len0 r1 `star` mlist r1 len1 r2)
+      (requires fun h0 ->
+        sel_list r0 len r2 h0 == L.(l0@l1) /\
+        L.length l0 = len0 /\ L.length l1 = len1)
+      (ensures  fun _ r1 h1 ->
+        sel_list r0 len0 r1 h1 == l0 /\
+        sel_list r1 len1 r2 h1 == l1)
+      (decreases len0)
+  =
+    if len0 = 0
+    then begin
+      intro_mlist_nil r0;
+        mlist_rew_len r0 0 len0 r0;
+      change_equal_slprop (mlist r0 len r2) (mlist r0 len1 r2);
+      r0
+    end else begin
+      let len'  = len  - 1 in
+      let len0' = len0 - 1 in
+        mlist_rew_len r0 len (len'+1) r2;
+      let r0' = elim_mlist_cons r0 len' r2 in
+      let r1  = elim_mlist_append r0' len' len0' len1 r2 (L.tl l0) l1 in
+      intro_mlist_cons r0 r0' len0' r1;
+        mlist_rew_len r0 (len0'+1) len0 r1;
+      r1
+    end
+
+
+(* [mlistN] *)
+
+type mlistN_sel_t (#a : Type) (entry : ref (cell a)) =
+  l : list (ref (cell a) & a) {sg_entry l null == entry}
+
+val mlistN_sl (#a : Type0) (entry : ref (cell a)) : slprop u#1
+
+val mlistN_sel (#a : Type) (entry : ref (cell a))
+  : selector (mlistN_sel_t entry) (mlistN_sl #a entry)
+
+[@@ __steel_reduce__]
+let mlistN' #a entry : vprop' = {
+  hp  = mlistN_sl    #a entry;
+  t   = mlistN_sel_t #a entry;
+  sel = mlistN_sel   #a entry
+}
+unfold let mlistN #a entry : vprop = VUnit (mlistN' #a entry)
+
+[@@ __steel_reduce__]
+let sel_listN (#a:Type0) (#p:vprop) (entry:ref (cell a))
+  (h:rmem p{FStar.Tactics.with_tactic selector_tactic (can_be_split p (mlistN entry) /\ True)})
+  : GTot (mlistN_sel_t #a entry)
+  = h (mlistN entry)
+
+val intro_mlistN (#a:Type) (#opened:inames) (entry:ref (cell a)) (len : nat)
+  : SteelGhost unit opened
+      (mlist #a entry len null) (fun () -> mlistN entry)
+      (requires fun _ -> True) (ensures fun h0 () h1 -> sel_listN entry h1 == sel_list entry len null h0)
+
+val elim_mlistN (#a:Type) (#opened:inames) (entry:ref (cell a))
+  : SteelGhost (G.erased nat) opened
+      (mlistN #a entry) (fun len -> mlist entry len null)
+      (requires fun _ -> True) (ensures fun h0 len h1 -> sel_list entry len null h1 == sel_listN entry h0)
+
+let intro_mlistN_nil #a #opened (r0 : ref (cell a))
+  : SteelGhost unit opened
+      emp (fun () -> mlistN #a r0)
+      (requires fun _ -> r0 == null) (ensures fun _ () h1 -> sel_listN #a r0 h1 == [])
+  = 
+    intro_mlist_nil #a null;
+    intro_mlistN #a null 0;
+    change_equal_slprop (mlistN #a null) (mlistN #a r0)
+
+(* TODO: use? *)
+let slabsurd (#a : Type) (#opened:inames) (#p : vprop) (#q : a -> vprop) ()
+  : SteelGhost a opened p q (requires fun _ -> False) (ensures fun _ _ _ -> True)
+  = let rt : a = () in
+    change_equal_slprop p (q rt);
+    rt
+
+let elim_mlistN_nil #a #opened r0
+  : SteelGhost unit opened
+      (mlistN #a r0) (fun () -> emp)
+      (requires fun _ -> r0 == null) (ensures fun h0 () _ -> sel_listN r0 h0 == [])
+  = let len = elim_mlistN r0 in
+    if len > 0 then entry_not_null r0 len null else noop (); (* need a else branch *)
+      mlist_rew_len r0 len 0 null;    
+    elim_mlist_nil r0 null
+
+let intro_mlistN_cons #a #opened r0 r1
+  : SteelGhost unit opened
+     (vptr r0 `star` mlistN #a r1)
+     (fun () -> mlistN r0)
+     (requires fun h0       -> (sel r0 h0).next == r1)
+     (ensures  fun h0 () h1 -> sel_listN r0 h1
+                            == (r0, (sel r0 h0).data) :: sel_listN r1 h0)
+  = let len = elim_mlistN r1 in
+    intro_mlist_cons r0 r1 len null;
+    intro_mlistN r0 (len+1)
+
+let elim_mlistN_cons #a #opened r0 hd tl
+  : SteelGhost (G.erased (ref (cell a))) opened
+     (mlistN r0)
+     (fun r1 -> vptr r0 `star` mlistN r1)
+     (requires fun h0 -> sel_listN r0 h0 == hd :: tl)
+     (ensures  fun h0 r1 h1 ->
+       G.reveal r1 == sg_entry tl null /\
+       sel r0 h1 == {next = r1; data = hd._2} /\
+       sel_listN r1 h1 == tl)
+  = let len = elim_mlistN r0 in
+      mlist_rew_len r0 len ((len-1)+1) null;
+    let r1 = elim_mlist_cons r0 (len-1) null in
+    intro_mlistN r1 (len-1);
+    r1
+
+
+let mlistN_entry_null_iff #a #opened entry
+  : SteelGhost unit opened
+      (mlistN #a entry) (fun () -> mlistN #a entry)
+      (requires fun _ -> True)
+      (ensures  fun h0 () h1 -> frame_equalities (mlistN #a entry) h0 h1 /\
+                             (is_null entry <==> Nil? (sel_listN entry h0)))
+  =
+    let l : G.erased (mlistN_sel_t entry) = gget (mlistN entry) in
+    match G.reveal l with
+    | [] -> US.noop_p (mlistN entry)
+    | hd :: tl ->
+      let r1 = elim_mlistN_cons entry hd tl in
+      vptr_not_null entry;
+      intro_mlistN_cons entry r1
+
+
+(* non-ghost functions *)
+
+inline_for_extraction
+let listN_is_nil #a (r0 : ref (cell a))
+  : Steel  bool
+          (mlistN #a r0) (fun _ -> mlistN #a r0)
+          (requires fun _ -> True)
+          (ensures  fun h0 b h1 ->
+                    frame_equalities (mlistN #a r0) h0 h1 /\
+                    b = is_null r0 /\
+                    (~b ==> Cons? (sel_listN r0 h0)) /\
+                    (b ==> sel_listN r0 h0 == []))
+  = 
+    (**) mlistN_entry_null_iff r0;
+    return (is_null #(cell a) r0)
+
+inline_for_extraction
+let list_next #a (r0 : ref (cell a)) (len : G.erased nat) (exit : G.erased (ref (cell a)))
+  : Steel (ref (cell a))
+          (mlist r0 (len + 1) exit) (fun r1 -> vptr r0 `star` mlist r1 len exit)
+          (requires fun _ -> True)
+          (ensures  fun h0 r1 h1 ->
+                   (let l = sel_list r0 (len+1) exit h0 in
+                    r1 == sg_entry (L.tl l) exit /\
+                    sel r0 h1 == {next = r1; data = (L.hd l)._2} /\
+                    sel_list r1 len exit h1 == L.tl l))
+  =
+    (**) let g_r1 : G.erased (ref (cell a)) = elim_mlist_cons r0 len exit in
+    let c0 = read r0 in
+    (**) change_equal_slprop (mlist (G.reveal g_r1) (G.reveal len) (G.reveal exit))
+    (**)                     (mlist c0.next (G.reveal len) (G.reveal exit));
+    return c0.next
+
+inline_for_extraction
+let listN_next #a (r0 : ref (cell a))
+  : Steel (ref (cell a))
+          (mlistN r0) (fun r1 -> vptr r0 `star` mlistN r1)
+          (requires fun h0       -> Cons? (sel_listN r0 h0))
+          (ensures  fun h0 r1 h1 ->
+                   (let l = sel_listN r0 h0 in 
+                    Cons? l /\ (* ?need to recall the requires *)
+                    r1 == sg_entry (L.tl l) null /\
+                    sel r0 h1 == {next = r1; data = (L.hd l)._2} /\
+                    sel_listN r1 h1 == L.tl l))
+  = 
+    (**) let l : G.erased (mlistN_sel_t r0) = gget (mlistN r0) in
+    (**) let g_r1 = elim_mlistN_cons r0 (L.hd l) (L.tl l) in
+    let c0 = read r0 in
+    (**) change_equal_slprop (mlistN (G.reveal g_r1)) (mlistN c0.next);
+    return c0.next
