steel/Learn.Steel.List.Impl.fst
@@ -1,0 +1,84 @@
+module Learn.Steel.List.Impl
+
+module L   = FStar.List.Pure
+module Ll  = Learn.List
+module G   = FStar.Ghost
+module U32 = FStar.UInt32
+
+open Steel.Effect
+open Steel.Effect.Atomic
+open Steel.Reference
+
+open Learn.Steel.List.DataD
+open Learn.Steel.List.Data
+open Learn.Steel.List.Derived
+
+
+let rec length (#a : Type) (r : ref (cell a))
+  : Steel  U32.t
+          (mlistN r) (fun _ -> mlistN r)
+          (requires fun h0        -> L.length (sel_listN r h0) <= FStar.UInt.max_int U32.n)
+          (ensures  fun h0 len h1 -> frame_equalities (mlistN r) h0 h1 /\
+                                  U32.v len = L.length (sel_listN r h0))
+  =
+    let b  = listN_is_nil r in
+    if b
+    then return 0ul
+    else begin
+      let r'   = listN_next r in
+      let len' = length r'    in
+      (**) intro_mlistN_cons r r';
+      return U32.(len' +^ 1ul)
+    end
+
+
+let rec insert_aux (#a : Type) (i : U32.t) (x : ref (cell a))
+                   (entry : ref (cell a)) (len : G.erased nat) (exit : G.erased (ref (cell a)))
+  : Steel  unit
+          (vptr x `star` mlist entry len exit) (fun () -> mlist entry (len+1) exit)
+          (requires fun _        -> 1 <= U32.v i /\ U32.v i <= len)
+          (ensures  fun h0 () h1 -> U32.v i <= len /\
+                                 sel_list entry (len+1) exit h1
+                                   == Ll.insert (U32.v i) (x, (sel x h0).data) (sel_list entry len exit h0))
+  =
+    (**) let len1 = G.hide (len - 1) in
+    (**) mlist_rew_len entry len (len1+1) exit;
+    let nxt = list_next entry len1 exit in
+    if U32.v i = 1
+    then begin
+      let x_c = read x in
+      write x ({x_c with next = nxt});
+      (**) intro_mlist_cons x nxt len1 exit;
+      let entry_c = read entry in
+      write entry ({entry_c with next = x});
+      (**) intro_mlist_cons entry x (len1+1) exit
+    end else begin
+      insert_aux U32.(i -^ 1ul) x nxt len1 exit;
+      (**) intro_mlist_cons entry nxt (len1+1) exit
+    end;
+    (**) mlist_rew_len entry ((len1+1)+1) (len+1) exit
+
+let insert (#a : Type) (i : U32.t) (x : ref (cell a))
+           (entry : ref (cell a)) (len : G.erased nat) (exit : G.erased (ref (cell a)))
+  : Steel (ref (cell a))
+          (vptr x `star` mlist entry len exit) (fun rt -> mlist rt (len+1) exit)
+          (requires fun _        -> U32.v i <= len)
+          (ensures  fun h0 rt h1 -> U32.v i <= len /\
+                                 sel_list rt (len+1) exit h1
+                                   == Ll.insert (U32.v i) (x, (sel x h0).data) (sel_list entry len exit h0))
+  =
+    if i = 0ul then begin
+      let x_c = read x in
+      write x ({x_c with next = entry});
+      (**) intro_mlist_cons x entry len exit;
+      return x
+    end else begin
+      insert_aux i x entry len exit;
+      entry
+    end
+
+
+(* ----------------- *)
+
+let length_u32 = length #U32.t
+let insert_u32 = insert #U32.t
