steel/Learn.Steel.Util.fst
@@ -1,0 +1,210 @@
+module Learn.Steel.Util
+
+module G = FStar.Ghost
+module Mem = Steel.Memory
+
+open Steel.Memory
+open Steel.Effect.Common
+open Steel.Effect.Atomic
+open FStar.Classical.Sugar
+open Steel.FractionalPermission
+open Steel.Reference
+
+#set-options "--ide_id_info_off"
+
+let pts_to_ref_injective_and
+      (#a:Type u#0) (r:ref a)
+      (p:perm)   (v0 v1:a) (m:mem)
+  : Lemma
+    (requires interp (pts_to_sl r p v0) m /\ interp (pts_to_sl r p v1) m)
+    (ensures  v0 == v1)
+  = pts_to_witinv r p;
+    Mem.elim_wi (pts_to_sl r p) v0 v1 m
+
+let return_ghost (#a:Type u#a) (#opened:inames)
+  (#p:a -> vprop)
+  (x:a)
+  : SteelGhostBase a true opened Unobservable
+         (return_pre (p x)) p
+         (return_req (p x)) (return_ens a x p)
+  = SteelGhostBase?.reflect (return_ a x opened #p)
+
+let noop_p (#opened) (p : vprop)
+  : SteelGhost unit opened p (fun () -> p) (fun _ -> True) (fun h0 () h1 -> frame_equalities p h0 h1)
+  = noop ()
+
+(* [vexists] *)
+(* TODO? $args *)
+
+let vexists_indep (#a : Type) (v : a -> vprop) (#t : Type) (f : (x:a) -> normal (t_of (v x)) -> GTot t)
+  : Tot prop
+  = forall (x0 x1 : a) (m : mem) .
+      interp (hp_of (v x0)) m /\ interp (hp_of (v x1)) m ==>
+      f x0 (sel_of (v x0) m) == f x1 (sel_of (v x1) m)
+
+let vexists_indepD (#a : Type) (v : a -> vprop) (#t : Type) (f : (x:a) -> normal (t_of (v x)) -> GTot t) 
+                   (x0 x1 : a) (m : mem)
+  : Lemma (requires vexists_indep #a v #t f /\
+                    interp (hp_of (v x0)) m /\ interp (hp_of (v x1)) m)
+          (ensures  f x0 (sel_of (v x0) m) == f x1 (sel_of (v x1) m))
+  = ()
+
+let vexists_indepI (#a : Type) (v : a -> vprop) (#t : Type) (f : (x:a) -> normal (t_of (v x)) -> GTot t)
+  (prf : (x0 : a) -> (x1 : a) -> (m : mem) ->
+         Lemma (requires interp (hp_of (v x0)) m /\ interp (hp_of (v x1)) m)
+               (ensures  f x0 (sel_of (v x0) m) == f x1 (sel_of (v x1) m)))
+  : Lemma (ensures vexists_indep #a v #t f)
+  = 
+    introduce forall (x0 x1 : a) (m : mem) . interp (hp_of (v x0)) m /\ interp (hp_of (v x1)) m ==>
+                                        f x0 (sel_of (v x0) m) == f x1 (sel_of (v x1) m)
+      with introduce _ ==> _
+      with _ . prf x0 x1 m
+
+let vexists_indepI_unique (#a : Type) (v : a -> vprop)
+  (prf : (x0 : a) -> (x1 : a) -> (m : mem) ->
+         Lemma (requires interp (hp_of (v x0)) m /\ interp (hp_of (v x1)) m)
+               (ensures  x0 == x1))
+  : Lemma (ensures forall (t : Type) (f : (x:a) -> normal (t_of (v x)) -> GTot t)
+                   . {:pattern (vexists_indep #a v #t f)}
+                     vexists_indep #a v #t f)
+  = introduce forall t f . vexists_indep #a v #t f
+      with vexists_indepI #a v #t f prf
+
+
+let vexists_sl (#a : Type) (v : a -> vprop)
+  : slprop
+  = Mem.h_exists #a (fun x -> hp_of (v x))
+
+let vexists_sel' (#a : Type) (v : a -> vprop) (#t : Type) (f : (x:a) -> t_of (v x) -> GTot t)
+  : selector' t (vexists_sl #a v)
+  = fun m ->
+      let x = Mem.id_elim_exists (fun x -> hp_of (v x)) m in
+      f x (sel_of (v x) m)
+
+let vexists_sel_depends_only_on
+      (#a : Type) (v : a -> vprop) (#t : Type) (f : (x:a) -> t_of (v x) -> GTot t)
+      (_ : squash (vexists_indep v f))
+      (m0 : Mem.hmem (vexists_sl v)) (m1 : mem{disjoint m0 m1})
+  : Lemma (vexists_sel' v f m0 == vexists_sel' v f (join m0 m1))
+  =
+    let x0 = G.reveal (Mem.id_elim_exists (fun x -> hp_of (v x))      m0     )  in
+    let x1 = G.reveal (Mem.id_elim_exists (fun x -> hp_of (v x)) (join m0 m1))  in
+    calc (==) {
+      vexists_sel' v f m0;
+    == {}
+      f x0 (sel_of (v x0) m0);
+    == {(* [sel_depends_only_on (sel_of (v x0))] *)}
+      f x0 (sel_of (v x0) (join m0 m1));
+    == { vexists_indepD v f x0 x1 (join m0 m1)}
+      f x1 (sel_of (v x1) (join m0 m1));
+    == {}
+      vexists_sel' v f (join m0 m1);
+    }
+
+let vexists_sel_depends_only_on_core
+      (#a : Type) (v : a -> vprop) (#t : Type) (f : (x:a) -> t_of (v x) -> GTot t)
+      (_ : squash (vexists_indep v f))
+      (m0 : Mem.hmem (vexists_sl v))
+  : Lemma (ensures  vexists_sel' v f m0 == vexists_sel' v f (core_mem m0))
+  =
+    let x0 = G.reveal (Mem.id_elim_exists (fun x -> hp_of (v x))      m0     )  in
+    let x1 = G.reveal (Mem.id_elim_exists (fun x -> hp_of (v x)) (core_mem m0)) in
+    calc (==) {
+      vexists_sel' v f m0;
+    == {}
+      f x0 (sel_of (v x0) m0);
+    == {(* [sel_depends_only_on_core (sel_of (v x0))] *)}
+      f x0 (sel_of (v x0) (core_mem m0));
+    == { vexists_indepD v f x0 x1 (core_mem m0)}
+      f x1 (sel_of (v x1) (core_mem m0));
+    == {}
+      vexists_sel' v f (core_mem m0);
+    }
+
+let vexists_sel (#a : Type) (v : a -> vprop) (#t : Type) (f : (x:a) -> normal (t_of (v x)) -> GTot t)
+  : Pure (selector t (vexists_sl #a v))
+         (requires vexists_indep v f) (ensures fun _ -> True)
+  =
+    Classical.forall_intro_2 (vexists_sel_depends_only_on      v f ());
+    Classical.forall_intro   (vexists_sel_depends_only_on_core v f ());
+    vexists_sel' v f
+
+[@__steel_reduce__]
+let vexists' (#a : Type) (v : a -> vprop) (#t : Type) (f : (x:a) -> normal (t_of (v x)) -> GTot t)
+  : Pure vprop' (requires vexists_indep v f) (ensures fun _ -> True)
+  = {
+    hp  = vexists_sl  v;
+    t   = t;
+    sel = vexists_sel v f
+  }
+
+[@__steel_reduce__]
+let vexists (#a : Type) (v : a -> vprop) (#t : Type) (f : (x:a) -> normal (t_of (v x)) -> GTot t)
+  : Pure vprop (requires vexists_indep v f) (ensures fun _ -> True)
+  = VUnit (vexists' v f)
+
+
+let intro_vexists_lem (#a : Type) (x : a) (v : a -> vprop)
+                      (#t : Type) (f : (x:a) -> normal (t_of (v x)) -> GTot t)
+                      (m : mem)
+  : Lemma (requires vexists_indep v f /\
+                    interp (hp_of (v x)) m)
+          (ensures  interp (hp_of (vexists v f)) m /\
+                    vexists_sel v f m == f x (sel_of (v x) m))
+  =
+    intro_h_exists x (fun x -> hp_of (v x)) m;
+    let x' = G.reveal (Mem.id_elim_exists (fun x -> hp_of (v x)) m) in
+    calc (==) {
+      vexists_sel v f m;
+    == {}
+      f x' (sel_of (v x') m);
+    == {vexists_indepD v f x x' m}
+      f x  (sel_of (v x) m);
+    }
+
+let intro_vexists (#a : Type) #opened (x : a) (v : a -> vprop)
+                  (#t : Type) (f : ((x:a) -> normal (t_of (v x)) -> GTot t) {vexists_indep v f})
+  : SteelGhost  unit opened
+               (v x)      (fun () -> vexists v f)
+               (fun _ -> True) (fun h0 () h1 -> h1 (vexists v f) == f x (h0 (v x)))
+  = change_slprop_rel
+      (v x) (vexists v f)
+      (fun y z -> z == f x y)
+      (intro_vexists_lem x v f)
+
+let witness_vexists_lem (#a : Type) (v : a -> vprop)
+                        (#t : Type) (f : (x:a) -> normal (t_of (v x)) -> GTot t)
+                        (m : mem)
+  : Ghost  a
+          (requires vexists_indep v f /\
+                    interp (hp_of (vexists v f)) m)
+          (ensures fun x ->
+                    interp (hp_of (v x)) m /\
+                    vexists_sel v f m == f x (sel_of (v x) m))
+  =
+    Mem.id_elim_exists (fun x -> hp_of (v x)) m
+
+let witness_vexists (#a : Type) #opened (v : a -> vprop)
+                    (#t : Type) (f : ((x:a) -> normal (t_of (v x)) -> GTot t) {vexists_indep v f})
+  : SteelGhost (G.erased a) opened
+               (vexists v f) (fun x -> v x)
+               (fun _ -> True)    (fun h0 x h1 -> h0 (vexists v f) == f x (h1 (v x)))
+  =
+    let z : G.erased t = gget (vexists v f) in
+    let rfn (x : a) (y : t_of (v x)) : prop = G.reveal z == f x y in
+    let lem (m : mem) : Lemma
+      (requires interp (hp_of (vexists v f)) m /\ sel_of (vexists v f) m == G.reveal z)
+      (ensures  interp (hp_of (h_exists #a (fun x -> v x `vrefine` rfn x))) m)
+      = let x = witness_vexists_lem v f m in
+        interp_vrefine_hp (v x) (rfn x) m;
+        assert (interp (hp_of (v x `vrefine` rfn x)) m);
+        Mem.intro_h_exists x (fun x -> hp_of (v x `vrefine` rfn x)) m;
+        assert_norm (interp (hp_of (h_exists #a (fun x -> v x `vrefine` rfn x))) m
+                  <==> interp (Mem.h_exists #a (fun x -> hp_of (v x `vrefine` rfn x))) m)
+    in
+    change_slprop
+      (vexists v f) (h_exists #a (fun x -> v x `vrefine` rfn x))
+      z () lem;
+    let x : G.erased a = witness_exists () in
+    elim_vrefine (v x) (rfn x);
+    x
